Clean/Air/OrderedChannel.lean
@@ -1,7 +1,7 @@
 import Clean.Air.FlatEnsemble
 
 variable {F : Type} [FiniteField F]
-open Air.Flat (Component Table Tables)
+open Air.Flat (Component Table TableContext)
 
 -- TODO deduplicate and add to Basic
 attribute [circuit_norm] forall_eq_or_imp List.mem_flatMap List.mem_map exists_exists_and_eq_and
@@ -189,7 +189,7 @@ where we assume our interactions are a subset of some larger list which is balan
 
 designed to be used for proving soundness by adding one table after another.
 -/
-def PartialBalancedChannel [DecidableEq F] (tables : Tables F) (channel : RawChannel F) : Prop :=
+def PartialBalancedChannel [DecidableEq F] (tables : TableContext F) (channel : RawChannel F) : Prop :=
   -- `extraInteractions` represents the unknown interactions from tables added later
   ∃ extraInteractions : List (Interaction F),
     -- the total of known + unknown interactions is balanced
@@ -204,7 +204,7 @@ def PartialBalancedChannel [DecidableEq F] (tables : Tables F) (channel : RawCha
     (channel ∉ tables.tables.flatMap (·.channelsWithGuarantees) ∨ ∀ i ∈ extraInteractions, i.Requirements tables.data)
 
 /-- Partial balance is trivially weaker than balance -/
-lemma partialBalancedChannel_of_balancedInteractions [DecidableEq F] {tables : Tables F} {channel : RawChannel F} :
+lemma partialBalancedChannel_of_balancedInteractions [DecidableEq F] {tables : TableContext F} {channel : RawChannel F} :
     BalancedInteractions (tables.interactionsWith channel) → PartialBalancedChannel tables channel := by
   intro balanced
   use []
@@ -214,15 +214,15 @@ lemma partialBalancedChannel_of_balancedInteractions [DecidableEq F] {tables : T
 For ordered channels, we can always instantiate partial balance at an initial sublist.
 -/
 theorem partialBalancedChannel_of_cons_of_orderedChannelLt [DecidableEq F]
-  {table : Table F} {tables : Tables F} (same_data : table.data = tables.data)
+  {table : Table F} {tables : TableContext F} (consistent : table.DataConsistency tables.data)
   {channel : RawChannel F} :
-  table.Constraints →
-  PartialBalancedChannel (.cons table tables same_data) channel →
+  table.Constraints tables.data →
+  PartialBalancedChannel (.cons table tables consistent) channel →
   OrderedChannelLt channel tables.components [table.component] →
     PartialBalancedChannel tables channel := by
   rintro table_constraints ⟨ extraInteractions, balanced, same_channel, extra_reqs_or_no_grts ⟩
     not_in_reqs_or
-  use table.interactionsWith channel ++ extraInteractions
+  use table.interactionsWith tables.data channel ++ extraInteractions
   simp only [circuit_norm] at *
   simp [or_imp] at ⊢ not_in_reqs_or extra_reqs_or_no_grts
   constructor
@@ -238,22 +238,23 @@ theorem partialBalancedChannel_of_cons_of_orderedChannelLt [DecidableEq F]
   rcases extra_reqs_or_no_grts with no_grts | extra_reqs
   · simp_all
   · right
-    have channel_reqs := table.requirements_of_not_mem_of_constraints table_constraints channel_not_in_reqs
-    rw [Table.channelRequirements_iff_forall, same_data] at channel_reqs
+    have channel_reqs := table.requirements_of_not_mem_of_constraints tables.data
+      table_constraints channel_not_in_reqs
+    rw [Table.channelRequirements_iff_forall] at channel_reqs
     exact ⟨ channel_reqs, extra_reqs ⟩
 
 /--
 For ordered channels, we can always instantiate partial balance at an initial sublist.
 -/
 lemma partialBalancedChannel_of_cons_of_orderedChannel [DecidableEq F]
-  {table : Table F} {tables : Tables F} (same_data : table.data = tables.data)
+  {table : Table F} {tables : TableContext F} (consistent : table.DataConsistency tables.data)
   {channel : RawChannel F} :
-  table.Constraints →
-  PartialBalancedChannel (tables.cons table same_data) channel →
+  table.Constraints tables.data →
+  PartialBalancedChannel (tables.cons table consistent) channel →
   OrderedChannel channel (table.component :: tables.components) →
     PartialBalancedChannel tables channel := by
   intro table_constraints partial_balance ordered_channel
-  apply partialBalancedChannel_of_cons_of_orderedChannelLt same_data table_constraints partial_balance
+  apply partialBalancedChannel_of_cons_of_orderedChannelLt consistent table_constraints partial_balance
   simp_all [circuit_norm]
 
 /--
@@ -262,15 +263,15 @@ on a list of tables by induction. This lemma captures the main step.
 -/
 lemma guarantees_of_requirements_cons [DecidableEq F]
   -- given a list of tables, and one additional table
-  {table : Table F} {tables : Tables F} (same_data : table.data = tables.data)
+  {table : Table F} {tables : TableContext F} (consistent : table.DataConsistency tables.data)
   -- and a channel that is consistent, ordered on the new table, and partially balanced on the combined tables
   {channel : RawChannel F} [channel.Consistent] :
-  table.Constraints →
+  table.Constraints tables.data →
   OrderedChannelRefl channel table.component →
-  PartialBalancedChannel (tables.cons table same_data) channel →
+  PartialBalancedChannel (tables.cons table consistent) channel →
   -- the channel requirements on the old tables imply guarantees on the new table
-  (∀ table ∈ tables.tables, table.ChannelRequirements channel) →
-    table.ChannelGuarantees channel := by
+  (∀ table ∈ tables.tables, table.ChannelRequirements tables.data channel) →
+    table.ChannelGuarantees tables.data channel := by
   rintro table_constraints ordered_channel partial_balance ih
   /-
   thanks to ordered channel, we know that channel cannot add _both_ grts and reqs for the new table.
@@ -280,18 +281,18 @@ lemma guarantees_of_requirements_cons [DecidableEq F]
   -/
   simp only [circuit_norm] at ordered_channel
   rcases ordered_channel with grts | reqs
-  · exact table.guarantees_of_not_mem grts
-  replace reqs := table.requirements_of_not_mem_of_constraints table_constraints reqs
+  · exact table.guarantees_of_not_mem tables.data grts
+  replace reqs := table.requirements_of_not_mem_of_constraints tables.data table_constraints reqs
   -- there's a special case to discard where the guarantees are trivially satisfied
   rcases partial_balance with ⟨ extraInteractions, balanced, same_channel, grts | extra_reqs ⟩
   · simp only [circuit_norm] at grts
-    exact table.guarantees_of_not_mem grts.left
+    exact table.guarantees_of_not_mem tables.data grts.left
   -- now, to prove this table's channel guarantees, we show guarantees on _all_ channel interactions (that we know are balanced)
-  set channelInteractions := (tables.cons table same_data).interactionsWith channel ++ extraInteractions
-  have subset_channelInteractions : table.interactionsWith channel ⊆ channelInteractions := by
+  set channelInteractions := (tables.cons table consistent).interactionsWith channel ++ extraInteractions
+  have subset_channelInteractions : table.interactionsWith tables.data channel ⊆ channelInteractions := by
     simp only [channelInteractions, circuit_norm]
   suffices all_grts : ∀ i ∈ channelInteractions, i.Guarantees tables.data by
-    rw [Table.channelGuarantees_iff_forall, same_data]
+    rw [Table.channelGuarantees_iff_forall]
     intro i hi
     exact all_grts i (subset_channelInteractions hi)
   -- this works since we can prove all channel _requirements_
@@ -301,13 +302,12 @@ lemma guarantees_of_requirements_cons [DecidableEq F]
     intro i h_mem
     rcases h_mem with h_mem_table | h_mem_old | h_mem_extra
     -- for the new table, we can just use the requirements assumption
-    · rw [Table.channelRequirements_iff_forall, same_data] at reqs
+    · rw [Table.channelRequirements_iff_forall] at reqs
       use table.channel_eq_of_mem_interactionsWith h_mem_table
       exact reqs _ h_mem_table
     · obtain ⟨ table', h_table', i_mem_table ⟩ := h_mem_old
       simp only [Table.channelRequirements_iff_forall] at ih
       specialize ih table' h_table'
-      simp only [tables.same_data _ h_table'] at ih
       use table'.channel_eq_of_mem_interactionsWith i_mem_table
       exact ih i i_mem_table
     · exact ⟨ same_channel i h_mem_extra, extra_reqs i h_mem_extra ⟩
@@ -319,16 +319,17 @@ lemma guarantees_of_requirements_cons [DecidableEq F]
 Partial balance can be specialized to a sublist (= part of a permutation),
 as long as none of the extra tables add requirements.
 -/
-lemma partialBalancedChannel_of_sublist [DecidableEq F] {subtables tables : Tables F} {channel : RawChannel F} :
+lemma partialBalancedChannel_of_sublist [DecidableEq F] {subtables tables : TableContext F}
+  (data_eq : subtables.data = tables.data) {channel : RawChannel F} :
   PartialBalancedChannel tables channel →
   (∃ otherTables, tables.tables.Perm (subtables.tables ++ otherTables) ∧
-    (∀ table ∈ otherTables, table.Constraints) ∧
+    (∀ table ∈ otherTables, table.Constraints tables.data) ∧
     ∀ table ∈ otherTables, channel ∉ table.channelsWithRequirements) →
     PartialBalancedChannel subtables channel := by
   rintro ⟨ extraInteractions, balanced, same_channel, no_grts_or_extra_reqs ⟩ subset_tables
   obtain ⟨ otherTables, perm, otherConstraints, otherReqs ⟩ := subset_tables
   by_cases subtables_empty : subtables.tables = []
-  · simp [subtables_empty, circuit_norm, PartialBalancedChannel, Tables.interactionsWith]
+  · simp [subtables_empty, circuit_norm, PartialBalancedChannel, TableContext.interactionsWith]
     use []
     simp [BalancedInteractions, balanceOf]
     by_cases h : ringChar F = 0
@@ -337,13 +338,7 @@ lemma partialBalancedChannel_of_sublist [DecidableEq F] {subtables tables : Tabl
   have subtables_subset : subtables.tables ⊆ tables.tables := by
     have p := perm.symm.subset
     simp_all
-  have subtables_data : subtables.data = tables.data := by
-    have ⟨ one_subtable, h_one_subtable ⟩ : ∃ table, table ∈ subtables.tables := by
-      apply List.exists_mem_of_ne_nil
-      simp [subtables_empty]
-    rw [← subtables.same_data _ h_one_subtable,
-      tables.same_data _ (subtables_subset h_one_subtable)]
-  use otherTables.flatMap (·.interactionsWith channel) ++ extraInteractions
+  use otherTables.flatMap (·.interactionsWith tables.data channel) ++ extraInteractions
   simp_all only
   constructor; swap
   -- TODO this half is surprisingly long/annoying, maybe missing helper lemmas
@@ -366,13 +361,14 @@ lemma partialBalancedChannel_of_sublist [DecidableEq F] {subtables tables : Tabl
     have ht' : t ∈ tables.tables := by
       apply perm.symm.subset
       simp [ht]
-    rw [← tables.same_data _ ht', ← Table.channelRequirements_iff_forall]
-    apply Table.requirements_of_not_mem_of_constraints
+    rw [← Table.channelRequirements_iff_forall]
+    apply t.requirements_of_not_mem_of_constraints tables.data
     exact otherConstraints _ ht
     exact otherReqs _ ht
   -- balance
   apply balancedInteractions_of_perm balanced
-  simp only [Tables.interactionsWith]
+  simp only [TableContext.interactionsWith]
+  rw [data_eq]
   grw [← List.append_assoc, List.perm_append_right_iff, ← List.flatMap_append, perm.flatMap]
   exact fun _ _ => List.Perm.refl _
 
@@ -385,24 +381,30 @@ This is relevant later when we add VM channels on top of an already finished, so
 -/
 lemma guarantees_of_requirements_append [DecidableEq F]
   -- given two lists of tables
-  {ts ss : Tables F} (same_data : ts.data = ss.data)
+  {ts ss : TableContext F} (data_eq : ts.data = ss.data)
   -- and a channel that is consistent, _doesn't add requirements_ on the new tables,
   -- and is partially balanced on the combined tables
   {channel : RawChannel F} [channel.Consistent] :
-  (∀ table ∈ ts.tables, table.Constraints) →
+  (∀ table ∈ ts.tables, table.Constraints ts.data) →
   (∀ table ∈ ts.tables, channel ∉ table.component.circuit.channelsWithRequirements) →
-  PartialBalancedChannel (ts.append ss same_data) channel →
+  PartialBalancedChannel (ts.append ss data_eq) channel →
   -- the channel requirements on the old tables imply guarantees on the new tables
-  (∀ table ∈ ss.tables, table.ChannelRequirements channel) →
-    ∀ table ∈ ts.tables, table.ChannelGuarantees channel := by
+  (∀ table ∈ ss.tables, table.ChannelRequirements ss.data channel) →
+    ∀ table ∈ ts.tables, table.ChannelGuarantees ts.data channel := by
   -- we show that for each (t, ss) pair, the assumptions of `*_cons` hold
   rintro constraints reqs partial_balance ih table h_table
-  have same_data' : table.data = ss.data := by
-    rw [ts.same_data _ h_table, same_data]
-  apply guarantees_of_requirements_cons (tables := ss) same_data' (constraints _ h_table) ?_ ?_ ih
+  have consistent : table.DataConsistency ss.data := by
+    rw [← data_eq]
+    exact ts.data_consistent table h_table
+  rw [data_eq]
+  apply guarantees_of_requirements_cons (tables := ss) consistent ?_ ?_ ?_ ih
+  · rw [← data_eq]
+    exact constraints _ h_table
   · right; exact reqs _ h_table
   -- get partial balance by sublist/permutation argument
-  apply partialBalancedChannel_of_sublist partial_balance
+  apply partialBalancedChannel_of_sublist
+    (subtables := ss.cons table consistent) (tables := ts.append ss data_eq)
+    data_eq.symm partial_balance
   obtain ⟨ i, hi, h' ⟩ := List.getElem_of_mem h_table
   symm at h'; subst h'
   use ts.tables.eraseIdx i
@@ -418,24 +420,27 @@ lemma guarantees_of_requirements_append [DecidableEq F]
     apply reqs _ (List.mem_of_mem_eraseIdx ht')
 
 /-- Helper lemma that uses circuit soundness, to strengthen guarantees to include requirements -/
-lemma iff_guarantees_of_constraints {table : Table F} {finished : List (RawChannel F)} :
-  table.Assumptions →
-  table.Constraints →
+lemma iff_guarantees_of_constraints {table : Table F} {data : ProverData F}
+    {finished : List (RawChannel F)} :
+  table.DataConsistency data →
+  table.Assumptions data →
+  table.Constraints data →
   table.component.circuit.channelsWithGuarantees ⊆ finished →
-  ((table.Spec ∧ ∀ channel ∈ finished, table.ChannelGuarantees channel ∧ table.ChannelRequirements channel) ↔
-    ∀ channel ∈ finished, table.ChannelGuarantees channel) := by
-  intro assumptions constraints subset_finished
+  ((table.Spec data ∧ ∀ channel ∈ finished,
+      table.ChannelGuarantees data channel ∧ table.ChannelRequirements data channel) ↔
+    ∀ channel ∈ finished, table.ChannelGuarantees data channel) := by
+  intro consistent assumptions constraints subset_finished
   constructor; simp_all
   intro grts
-  have all_grts : table.Guarantees := by
+  have all_grts : table.Guarantees data := by
     rw [Table.guarantees_iff_channelGuarantees]
     intro channel h_channel
     exact grts _ (subset_finished h_channel)
   -- constraints ∧ guarantees → requirements → channelRequirements
-  have ⟨ spec, all_reqs ⟩ := table.weakSoundness assumptions constraints all_grts
+  have ⟨ spec, all_reqs ⟩ := table.weakSoundness consistent assumptions constraints all_grts
   use spec
   intro channel h_channel
-  exact ⟨ grts _ h_channel, table.channelRequirements_of_requirements all_reqs ⟩
+  exact ⟨ grts _ h_channel, table.channelRequirements_of_requirements data all_reqs ⟩
 
 /--
 `SoundChannels` combines three assumptions on the channels used by a list of tables,
@@ -463,29 +468,30 @@ def SoundChannels [DecidableEq F] (tables : List (Component F)) (finished : List
   ∀ channel ∈ finished, channel.Consistent
 
 /-- `SoundChannels` lets us prove a soundness theorem. -/
-theorem spec_and_guarantees_of_soundChannels [DecidableEq F] {witness : Tables F} {finished : List (RawChannel F)} :
+theorem spec_and_guarantees_of_soundChannels [DecidableEq F] {witness : TableContext F} {finished : List (RawChannel F)} :
   SoundChannels (witness.tables.map (·.component)) finished →
   -- constraints + partial balance
   witness.Assumptions →
   witness.Constraints →
   (∀ channel ∈ finished, PartialBalancedChannel witness channel) →
     -- implies the spec, and the guarantees and requirements on all finished channels
-    ∀ table ∈ witness.tables, table.Spec ∧ ∀ channel ∈ finished,
-    table.ChannelGuarantees channel ∧ table.ChannelRequirements channel := by
+    ∀ table ∈ witness.tables, table.Spec witness.data ∧ ∀ channel ∈ finished,
+    table.ChannelGuarantees witness.data channel ∧
+      table.ChannelRequirements witness.data channel := by
   -- by induction on the tables
   rintro ⟨ subset_finished, ordered_channels, consistent_channels ⟩ assumptions constraints partial_balance
-  induction witness using Tables.induct
+  induction witness using TableContext.induct
   · intro _ h_table; nomatch h_table
   -- induction step
-  rename_i table tables same_data ih
-  simp only [Tables.Assumptions, Tables.Constraints, circuit_norm] at *
+  rename_i table tables consistent ih
+  simp only [TableContext.Assumptions, TableContext.Constraints, circuit_norm] at *
   simp only [forall_exists_index, and_imp, forall_apply_eq_imp_iff₂] at *
   -- first, we use the IH
   have partial_balance' c hc := by
-    apply partialBalancedChannel_of_cons_of_orderedChannelLt same_data constraints.left
+    apply partialBalancedChannel_of_cons_of_orderedChannelLt consistent constraints.left
       (partial_balance c hc)
     rw [OrderedChannelLt]
-    simp only [Tables.components, List.flatMap_singleton]
+    simp only [TableContext.components, List.flatMap_singleton]
     rcases (ordered_channels c hc).2.2 with no_grts | no_reqs
     · left
       intro h_component
@@ -499,13 +505,13 @@ theorem spec_and_guarantees_of_soundChannels [DecidableEq F] {witness : Tables F
   constructor; swap
   · exact ih
   -- it's enough to prove guarantees of all channels, since they + constraints imply requirements
-  rw [iff_guarantees_of_constraints assumptions.left constraints.left subset_finished.left]
+  rw [iff_guarantees_of_constraints consistent assumptions.left constraints.left subset_finished.left]
   -- the rest is just applying `guarantees_of_requirements_cons`
   intro channel h_channel
   have : channel.Consistent := consistent_channels _ h_channel
   have orderedChannelRefl : OrderedChannelRefl channel table.component := by
     simp only [circuit_norm, ordered_channels channel h_channel]
-  apply guarantees_of_requirements_cons same_data
+  apply guarantees_of_requirements_cons consistent
     constraints.left orderedChannelRefl (partial_balance channel h_channel)
   intro t ht
   exact (ih t ht).right _ h_channel |>.right
@@ -550,7 +556,7 @@ namespace Ensemble
 lemma partialBalancedChannel_of_balancedChannel {ens : Ensemble F PublicIO}
     {witness : EnsembleWitness ens} (channel : RawChannel F) :
   witness.BalancedChannel channel →
-    PartialBalancedChannel witness channel := by
+    PartialBalancedChannel witness.tableContext channel := by
   intro balanced
   use []
   simp_all [EnsembleWitness.BalancedChannel]
@@ -572,11 +578,13 @@ theorem tableSoundness_of_soundChannels {ens : Ensemble F PublicIO} :
   (∃ finished, finished ⊆ ens.channels ∧ ens.SoundChannels finished) →
     ens.TableSoundness := by
   intro ⟨ finished, finished_subset, soundChannels ⟩ witness assumptions constraints balance table h_table
-  have partial_balance : ∀ channel ∈ finished, PartialBalancedChannel witness channel := by
+  have partial_balance : ∀ channel ∈ finished,
+      PartialBalancedChannel witness.tableContext channel := by
     intro channel h_channel
     apply partialBalancedChannel_of_balancedChannel
     exact balance _ <| finished_subset h_channel
-  apply spec_and_guarantees_of_soundChannels ?soundChannels ?assumptions ?constraints
+  apply spec_and_guarantees_of_soundChannels (witness := witness.tableContext)
+    ?soundChannels ?assumptions ?constraints
     partial_balance table h_table |>.left
   <;> (simp only [circuit_norm]; assumption)
 
